theories/L6_PCPS/lambda_lifting_corresp.v
@@ -65,7 +65,17 @@ Section Lambda_lifting_corresp.
     - now rewrite M.gss, extend_gss.
     - now rewrite M.gso, extend_gso.
   Qed.
-  
+
+  Lemma rename_set_WraperFun_f_eq m x y :
+    f_eq (rename (M.set x (WrapperFun y) m))
+         ((rename m) {x ~> y}).
+  Proof.
+    intros z. unfold rename.
+    destruct (peq z x); subst; simpl.
+    - now rewrite M.gss, extend_gss.
+    - now rewrite M.gso, extend_gso.
+  Qed.
+
   Lemma rename_not_in_domain_f_eq m x :
     ~ x \in Dom_map m ->
     f_eq (rename m) ((rename m) {x ~> x}).
@@ -87,7 +97,18 @@ Section Lambda_lifting_corresp.
       normalize_sets. intros Hc. eapply Hnin. constructor; eauto.
       normalize_sets. sets. 
   Qed.
-  
+
+  Lemma rename_not_in_domain_add_extend_fundefs_f_eq m B :
+    Disjoint _ (name_in_fundefs B) (Dom_map m) ->
+    f_eq (rename m) (alpha_conv.extend_fundefs (rename m) B B).
+  Proof with now eauto with Ensembles_DB.
+    induction B; intros Hnin; simpl; eauto.
+    - rewrite <- IHB. rewrite <- rename_not_in_domain_f_eq. reflexivity.
+      simpl in *. intros Hc. eapply Hnin. constructor; eauto.
+      sets.
+    - reflexivity.    
+  Qed.
+
   (** * Lemmas about [fun_map] *)
   
 
@@ -130,6 +151,7 @@ Section Lambda_lifting_corresp.
     intros. inv H. eassumption.
   Qed.
 
+
   (** [add_functions] is sound w.r.t. its relational spec *)
   Lemma add_functions_true_sound B fvs sfvs args fm gfuns fvm S :
     Disjoint _ (S :|: bound_var_fundefs B) (Dom_map fvm) ->
@@ -140,6 +162,8 @@ Section Lambda_lifting_corresp.
          let '(fm', gfuns') := m in
          exists σ ζ S',
            Add_functions B args (rename fvm) (fun_map fm) S σ ζ S' /\
+           name_in_fundefs B \subset (domain (fun_map fm')) /\
+           Dom_map fm' <--> Dom_map fm :|: name_in_fundefs B /\
            f_eq σ (rename fvm) /\
            f_eq ζ (fun_map fm') /\
            fresh S' (next_var (fst s')) }}.
@@ -152,6 +176,8 @@ Section Lambda_lifting_corresp.
         eapply pre_existential; intros g2.
         eapply pre_existential; intros S'.
         eapply pre_curry_l. intros Hadd.
+        eapply pre_curry_l. intros Hin.
+        eapply pre_curry_l. intros Hdom.
         eapply pre_curry_l. intros Hfeq1.
         eapply pre_curry_l. intros Hfeq2.
         rewrite Hbeq. 
@@ -163,9 +189,11 @@ Section Lambda_lifting_corresp.
                                                      (next_var (fst s2) < s)%positive /\
                                                      fresh (S' \\ [set x]) s).
         intros ft s3. apply return_triple. intros _ s4 Hf. destructAll.
-        do 3 eexists. split ; [| split; [| split ]].
+        do 3 eexists. split ; [| split; [| split; [| split; [| split ]]]].
         
         -- econstructor. eassumption. eassumption.
+        -- rewrite fun_map_set_Fun_f_eq. rewrite <- domain_extend_Some. sets. 
+        -- rewrite Dom_map_set. rewrite Hdom. sets.
         -- symmetry. rewrite Hfeq1, <- !rename_not_in_domain_f_eq. reflexivity.
            intros Hc. eapply Hnin. constructor; [| eassumption ]. left.
            eapply Add_functions_free_set_Included; eauto.
@@ -173,8 +201,9 @@ Section Lambda_lifting_corresp.
            now constructor.
         -- symmetry. rewrite Hfeq2. apply fun_map_set_Fun_f_eq.
         -- eassumption. 
-    - apply return_triple. intros s Hf.
-      repeat eexists; eauto. constructor; reflexivity.
+    - apply return_triple. intros _ s Hf.
+      do 3 eexists; eauto. split. constructor; reflexivity.
+      split. sets. split. simpl. sets. split. reflexivity. split. reflexivity. eassumption.
   Qed.
   
   Lemma add_functions_false_sound B fvs sfvs args fm gfuns S :
@@ -184,57 +213,152 @@ Section Lambda_lifting_corresp.
     {{ fun r s => fresh S (next_var (fst s)) }}
       add_functions B fvs sfvs args fm gfuns
     {{ fun r s m s' =>
-         let '(fm', gfuns') := m in
-         exists S',
-           Dom_map fm' <--> Dom_map fm :|: name_in_fundefs B /\
-           (* gfuns' = gfuns /\ *)
-           f_eq (fun_map fm) (fun_map fm') /\
-           fresh S' (next_var (fst s')) }}.
+         let '(fm', gfuns') := m in         
+         Dom_map fm' <--> Dom_map fm :|: name_in_fundefs B /\
+         Disjoint _ (name_in_fundefs B) (domain (fun_map fm')) /\
+         f_eq (fun_map fm) (fun_map fm') /\
+         fresh S (next_var (fst s')) }}.
   Proof with now eauto with Ensembles_DB.
     revert fm S. induction B; intros fm S Hdis Hun Hbeq.
     - eapply bind_triple.
       + eapply IHB.
         normalize_bound_var_in_ctx. now sets. inv Hun. eassumption.
         eassumption. 
-      + intros [fm' gfuns'] s1. simpl. eapply pre_existential; intros S'.
+      + intros [fm' gfuns'] s1. simpl.
         eapply pre_curry_l. intros Heq.
         (* eapply pre_curry_l. intros Hfeq1. *)
         rewrite Hbeq.  
         simpl. apply return_triple. intros _ s4 Hf. destructAll.
-        eexists. split; [| split ].
+        split; [| split; [| split ]].
         * rewrite Dom_map_set, Heq. now sets.
-        * symmetry. rewrite H; eauto. eapply fun_map_set_NoListFun_f_eq.
+        * eapply Union_Disjoint_l.
+          2:{ rewrite fun_map_set_NoListFun_f_eq. eassumption.
+              inv Hun.
+              intros Hc. eapply Heq in Hc. inv Hc; eauto.
+              eapply Hdis. constructor. now eauto. eassumption.
+              eapply H8. eapply name_in_fundefs_bound_var_fundefs. eassumption. }
+          eapply Disjoint_Singleton_l. intros Hc.
+          unfold domain, fun_map, In in *. destruct Hc. rewrite M.gss in H2. congruence.
+        * symmetry. rewrite H0; eauto. eapply fun_map_set_NoListFun_f_eq.
           intros Hnin. eapply Heq in Hnin. inv Hnin.
           -- eapply Hdis. constructor; eauto.
-          -- inv Hun; eauto. eapply H8. eapply name_in_fundefs_bound_var_fundefs.
+          -- inv Hun; eauto. eapply H9. eapply name_in_fundefs_bound_var_fundefs.
              eassumption.
         * eassumption.
     - apply return_triple. intros s Hf Hs.
-      eexists; eauto. split. simpl; now sets. split. reflexivity.
+      split. simpl; now sets. split. now sets.
+      split. reflexivity.
       eassumption.
+  Qed.
+
+  (** [make_wrappers] is sound *)
+
+  Lemma make_wrappers_sound_subset S B fv fm :
+    name_in_fundefs B \subset (domain (fun_map fm)) ->
+    {{ fun r s => fresh S (next_var (fst s)) }}
+      make_wrappers B fv fm 
+    {{ fun r s r s' =>
+         let (o, fv') := r in
+         exists B' σ S',
+           o = Some B' /\
+           Make_wrappers (fun_map fm) (rename fv) B S B' S' σ /\
+           f_eq (rename fv') σ /\
+           Dom_map fv' <--> name_in_fundefs B :|: Dom_map fv /\
+           fresh S' (next_var (fst s'))
+    }}.
+  Proof.
+    revert S; induction B; intros S Hsub.
+    - unfold make_wrappers.
+      destruct (fm ! v) eqn:Hget.
+      + destruct f0.
+        eapply bind_triple. eapply get_name_spec.
+        simpl. intros z [c u].
+        eapply pre_curry_l. intros Hf.
+        eapply bind_triple.
+        eapply frame_rule. eapply frame_rule.
+        now eapply get_names_lst_spec.
+        intros xs [c' u'].
+        eapply pre_curry_l. intros Hf'.
+        eapply pre_curry_l. intros Hlt.
+        eapply pre_curry_l. intros Hnd.
+        eapply pre_curry_l. intros Hlen.
+        eapply pre_curry_l. intros Hsub'.
+        eapply bind_triple.
+        * eapply frame_rule. eapply frame_rule.
+          eapply pre_strenghtening.
+          intros. rewrite Setminus_Union, Union_commut, <- Setminus_Union in H.
+          eapply H. eapply IHB.
+          eapply Included_trans; [| eassumption ]; sets.
+        * intros [C fv'] [c'' u'']. destruct C.
+          { eapply return_triple.
+            simpl; intros. destructAll.
+            do 3 eexists. split; [| split; [| split ]].
+            -- reflexivity. 
+            -- inv H1. econstructor; eauto.
+               unfold fun_map. rewrite Hget. reflexivity.
+               eapply Included_trans. eapply Hsub'. now sets.  
+               constructor; eauto. intros Hc. eapply Hsub'; eauto.
+            -- simpl. rewrite rename_set_WraperFun_f_eq. rewrite H3. reflexivity.
+            -- rewrite Dom_map_set, H4. sets. }
+          { eapply return_triple. simpl; intros. destructAll. congruence. }
+        * exfalso.
+          assert (Hin : domain (fun_map fm) v). eapply Hsub. now left.
+          destruct Hin. unfold fun_map in *. rewrite Hget in H. congruence.
+      + exfalso.
+        assert (Hin : domain (fun_map fm) v). eapply Hsub. now left.
+        destruct Hin. unfold fun_map in *. rewrite Hget in H. congruence.
+    - eapply return_triple. intros. do 3 eexists. split.
+      reflexivity. split. constructor. split. reflexivity. split. simpl. sets. eassumption.
+  Qed.
+
+  Lemma make_wrappers_sound_Disjoint S B fv fm :
+    B <> Fnil ->
+    name_in_fundefs B \subset Dom_map fm ->
+    Disjoint _ (name_in_fundefs B) (domain (fun_map fm)) ->
+    {{ fun r s => fresh S (next_var (fst s)) }}
+      make_wrappers B fv fm 
+    {{ fun r s r s' =>
+         let (o, fv') := r in
+         o = None /\
+         fv = fv' /\
+         fresh S (next_var (fst s'))
+    }}.
+  Proof.
+    intros Hneq Hin Hdis. destruct B.
+    - unfold make_wrappers.
+      destruct (fm ! v) eqn:Hget.
+      + destruct f0.
+        exfalso.
+        eapply Hdis. constructor. now left. eexists. unfold fun_map. rewrite Hget. reflexivity.
+        eapply return_triple. intros. split; eauto. 
+      + exfalso. 
+        assert (Hin' : Dom_map fm v). eapply Hin. now left.
+        destruct Hin'. congruence.
+    - congruence.
   Qed.
 
   (** [add_free_var] spec *)
   Lemma add_free_vars_f_eq xs fvm S P :
-    binding_not_in_map P fvm ->    
-    (* Disjoint _ (domain (fun_map m)) (FromList xs) -> *)
-    (* binding_not_in_map S m -> *)
-    {{ fun s => fresh S (next_var s) }}
+    Disjoint _ P (Dom_map fvm) ->
+    {{ fun r s => fresh S (next_var (fst s)) }}
       add_free_vars xs fvm
-    {{ fun s p s' =>
+    {{ fun r s p s' =>
          let (ys, fvm') := p in  
          f_eq ((rename fvm) <{xs ~> ys}>) (rename fvm') /\
-         binding_not_in_map (Setminus _ P (FromList xs)) fvm' /\
+         Disjoint _ (Setminus _ P (FromList xs)) (Dom_map fvm') /\
          NoDup ys /\
-         Forall (fresh S) ys /\
+         FromList ys \subset S /\
          length xs = length ys /\
-         fresh (Setminus var S (FromList ys)) (next_var s') }}.
+         fresh (Setminus var S (FromList ys)) (next_var (fst s')) }}.
   Proof with now eauto with Ensembles_DB.
     revert fvm S. induction xs as [| x xs IHxs ]; intros fvm S Hnin.
     - apply return_triple. simpl.
-      intros s Hf. repeat split; eauto.
-      eapply binding_not_in_map_antimon; eauto.
-      rewrite FromList_nil... now constructor.
+      intros r [w s] Hf. split. reflexivity. split.
+      normalize_sets. rewrite Setminus_Empty_set_neut_r. eassumption.
+      split. now constructor.
+      split. now sets.
+      split. reflexivity.
+      normalize_sets. rewrite Setminus_Empty_set_neut_r. eassumption.
     - eapply bind_triple.
       + eapply IHxs; eauto.
       + intros [ys m'] _.
@@ -244,19 +368,15 @@ Section Lambda_lifting_corresp.
         apply pre_curry_l. intros Hall.
         apply pre_curry_l. intros Hlen.
         eapply bind_triple. now apply get_name_spec.
-        intros y s1. apply return_triple. 
-        intros s2 [Hf1 Hf2]. split; [| split; [| split; [| split; [| split ]]]].
+        intros y [w1 s1]. apply return_triple. 
+        intros s2 [w2 s3] H. destructAll. split; [| split; [| split; [| split; [| split ]]]].
         * simpl. rewrite rename_set_FreeVar_f_eq, Hfeq1.
           reflexivity.
-        * eapply binding_not_in_map_set_not_In_S.
-          eapply binding_not_in_map_antimon; [| eassumption ].
-          rewrite FromList_cons...
-          intros Hc; inv Hc. eapply H0. rewrite FromList_cons...
-        * constructor; eauto. intros Hc.
-          specialize (Hf1 y (Pos.le_refl y)). inv Hf1.
-          eauto.
-        * constructor; eauto.
-          eapply fresh_monotonic; [| eassumption ]...
+        * normalize_sets. rewrite Dom_map_set. sets.
+        * constructor; eauto. intros Hc. simpl in *. 
+          eapply H. eassumption. 
+        * normalize_sets. eapply Union_Included; eauto.
+          inv H. eapply Singleton_Included. eassumption.
         * simpl; congruence.
         * rewrite FromList_cons, Union_commut, <- Setminus_Union. eassumption.
   Qed.
@@ -298,6 +418,25 @@ Section Lambda_lifting_corresp.
       constructor.
   Qed.
 
+
+  Lemma Make_wrappers_f_eq B B' S1 S2 σ1 ζ1 σ2 σ1' ζ1' :
+    Make_wrappers ζ1 σ1 B S1 B' S2 σ2 ->
+    f_eq σ1 σ1' ->
+    f_eq ζ1 ζ1' ->
+    exists σ2',
+      Make_wrappers ζ1' σ1' B S1 B' S2 σ2' /\
+      f_eq σ2 σ2'.
+  Proof.
+    intros Hadd. revert σ1' ζ1'.
+    induction Hadd; intros σ1' ζ1' Heq1 Heq2.
+    - eexists. split.
+      econstructor. eassumption.
+    - edestruct IHHadd as [σ2' [Hadd' Heq']]; eauto.
+      eexists. split.
+      rewrite Heq1. econstructor; eauto. rewrite <- Heq2. eassumption.
+      rewrite Heq'. reflexivity. 
+  Qed.
+
   (** * Some Proper instances *)
   
   Instance FunsFVs_Proper : Proper (f_eq ==> Same_set _) FunsFVs.
@@ -330,31 +469,69 @@ Section Lambda_lifting_corresp.
        (Hll : Exp_lambda_lift ζ σ e S1 e' S2)
        (Heq1 : f_eq σ σ') (Heq2 : f_eq ζ ζ'),
        Exp_lambda_lift ζ' σ' e S1 e' S2) /\
-    (forall B ζ σ ζ' σ' S1 B' S2
-       (Hll : Fundefs_lambda_lift ζ σ B S1 B' S2) (Heq1 : f_eq σ σ') (Heq2 : f_eq ζ ζ'),
-       Fundefs_lambda_lift ζ' σ' B S1 B' S2).
+    (forall B B0 ζ σ ζ' σ' S1 B' S2,
+        (forall (Hll : Fundefs_lambda_lift1 ζ σ B S1 B' S2) (Heq1 : f_eq σ σ') (Heq2 : f_eq ζ ζ'),
+            Fundefs_lambda_lift1 ζ' σ' B S1 B' S2) /\
+        (forall (Hll : Fundefs_lambda_lift2 ζ σ B0 B S1 B' S2) (Heq1 : f_eq σ σ') (Heq2 : f_eq ζ ζ'),
+            Fundefs_lambda_lift2 ζ' σ' B0 B S1 B' S2) /\
+        (forall (Hll : Fundefs_lambda_lift3 ζ σ B0 B S1 B' S2) (Heq1 : f_eq σ σ') (Heq2 : f_eq ζ ζ'),
+          Fundefs_lambda_lift3 ζ' σ' B0 B S1 B' S2)).    
   Proof.
-    eapply exp_def_mutual_ind; simpl; intros; inv Hll.
+    eapply exp_def_mutual_ind; simpl; intros; try inv Hll.
     - rewrite Heq1. econstructor; eauto. eapply H; eauto.
       rewrite Heq1; reflexivity.
     - rewrite Heq1. econstructor; eauto.
     - rewrite Heq1. econstructor; eauto.
     - rewrite Heq1. econstructor; eauto.
       eapply H; eauto. rewrite Heq1; reflexivity.
+    - rewrite !Heq1. eapply LL_Eletapp_known. 
+      rewrite <- Heq2. eassumption. 
+      eapply H; eauto.
+      rewrite Heq1; reflexivity.
+    - rewrite !Heq1. eapply LL_Eletapp_unknown. 
+      eapply H; eauto.
+      rewrite Heq1; reflexivity.
     - edestruct Add_functions_f_eq' as [σ'' [ζ'' [Hadd1 [Heq1' Heq2']]]]; eauto.
       econstructor. eapply Included_trans. eassumption.
       eapply Included_Union_compat. reflexivity.
-      eapply Included_Union_compat; rewrite <- Heq2; reflexivity.
+      eapply Included_Union_compat.
+      eapply FunsFVs_Proper. symmetry. eassumption.
+      eapply LiftedFuns_Proper. symmetry. eassumption.
       eassumption. eassumption. now eapply H; eauto.
       now eapply H0; eauto.
+    - edestruct Add_functions_f_eq' as [σ''' [ζ'' [Hadd1 [Heq1' Heq2']]]]; eauto.
+      edestruct Make_wrappers_f_eq as [σ2 [S2' Hwr]]. eassumption.
+      eassumption. eassumption. 
+      eapply LL_Efun2.
+      eapply Included_trans. eassumption.
+      eapply Included_Union_compat. reflexivity.
+      eapply Included_Union_compat.
+      eapply FunsFVs_Proper. symmetry. eassumption.
+      eapply LiftedFuns_Proper. symmetry. eassumption.
+      eassumption. eassumption.
+      eapply H; eassumption. eassumption.
+      eapply H0; eassumption.
+    - eapply LL_Efun3.
+      now eapply H; eauto.
+      eapply H0; eauto. rewrite Heq1. reflexivity.       
     - rewrite !Heq1. econstructor; eauto. rewrite <- Heq2. eauto.
     - rewrite !Heq1. econstructor; eauto.
     - rewrite Heq1. econstructor; eauto. eapply H; eauto.
       rewrite Heq1. reflexivity.
     - rewrite Heq1. econstructor; eauto.
-    - rewrite Heq1. econstructor; eauto. rewrite <- Heq2; eauto.
-      eapply H; eauto. rewrite Heq1. reflexivity.
-    - constructor.
+    - split; [| split ]; intros.
+      + inv Hll. rewrite Heq1. econstructor; eauto. rewrite <- Heq2; eauto.
+        eapply H; eauto. rewrite Heq1. reflexivity.
+        eapply H0; eauto.
+      + inv Hll.
+        edestruct Make_wrappers_f_eq as [σ2 [S2' Hwr]]. eassumption. rewrite Heq1. reflexivity.
+        eassumption. 
+        econstructor; eauto. rewrite <- Heq2; eauto.
+        eapply H0. eassumption. eassumption. eassumption.
+      + inv Hll. econstructor; eauto.
+        eapply H; eauto. rewrite Heq1. reflexivity.
+        eapply H0; eauto.
+    - split; [| split ]; intros; inv Hll; constructor.
   Qed.
 
   Instance Exp_lambda_lift_Proper_ζ :
@@ -373,21 +550,55 @@ Section Lambda_lifting_corresp.
     symmetry. eassumption.
   Qed.
 
-  Instance Fundefs_lambda_lift_Proper_ζ :
-    Proper (f_eq ==> eq ==> eq ==> eq ==> eq ==> eq ==> iff) Fundefs_lambda_lift.
+  Instance Fundefs_lambda_lift1_Proper_ζ :
+    Proper (f_eq ==> eq ==> eq ==> eq ==> eq ==> eq ==> iff) Fundefs_lambda_lift1.
   Proof.
     constructor; intros; subst;
     eapply Exp_lambda_lift_proper_mut; try eassumption; try reflexivity.
     symmetry. eassumption.
   Qed.
 
-  Instance Fundefs_lambda_lift_Proper_σ :
-    Proper (eq ==> f_eq ==> eq ==> eq ==> eq ==> eq ==> iff) Fundefs_lambda_lift.
+  Instance Fundefs_lambda_lift1_Proper_σ :
+    Proper (eq ==> f_eq ==> eq ==> eq ==> eq ==> eq ==> iff) Fundefs_lambda_lift1.
   Proof.
     constructor; intros; subst;
     eapply Exp_lambda_lift_proper_mut; try eassumption; try reflexivity.
     symmetry. eassumption.
   Qed.
+
+  Instance Fundefs_lambda2_lift_Proper_ζ :
+    Proper (f_eq ==> eq ==> eq ==> eq ==> eq ==> eq ==> eq ==> iff) Fundefs_lambda_lift2.
+  Proof.
+    constructor; intros; subst;
+    eapply Exp_lambda_lift_proper_mut; try eassumption; try reflexivity.
+    symmetry. eassumption.
+  Qed.
+
+  Instance Fundefs_lambda2_lift_Proper_σ :
+    Proper (eq ==> f_eq ==> eq ==> eq ==> eq ==> eq ==> eq ==> iff) Fundefs_lambda_lift2.
+  Proof.
+    constructor; intros; subst;
+    eapply Exp_lambda_lift_proper_mut; try eassumption; try reflexivity.
+    symmetry. eassumption.
+  Qed.
+  
+  Instance Fundefs_lambda3_lift_Proper_ζ :
+      Proper (f_eq ==> eq ==> eq ==> eq ==> eq ==> eq ==> eq ==> iff) Fundefs_lambda_lift3.
+  Proof.
+    constructor; intros; subst;
+    eapply Exp_lambda_lift_proper_mut; try eassumption; try reflexivity.
+    symmetry. eassumption.
+  Qed.
+
+  Instance Fundefs_lambda3_lift_Proper_σ :
+    Proper (eq ==> f_eq ==> eq ==> eq ==> eq ==> eq ==> eq ==> iff) Fundefs_lambda_lift3.
+  Proof.
+    constructor; intros; subst;
+    eapply Exp_lambda_lift_proper_mut; try eassumption; try reflexivity.
+    symmetry. eassumption.
+  Qed.
+
+
 
   (** Alternative definition for [Funs] *)
   Lemma Funs_Same_set ζ : 
@@ -418,14 +629,14 @@ Section Lambda_lifting_corresp.
     
     Variable (funmap : FunInfoMap).
 
-    Lemma exp_true_fv_fundefs_true_fv_correct :
+    Lemma exp_true_fv_fundefs_true_fv_correct lift_dec :
       (forall e Scope FVset x,
-         PS.In x (exp_true_fv_aux funmap e Scope FVset) ->
+         PS.In x (exp_true_fv_aux lift_dec funmap e Scope FVset) ->
          ((In _ (occurs_free e) x /\ ~ PS.In x Scope) \/
           (In _ (Union _ (FunsFVs (fun_map funmap)) (LiftedFuns (fun_map funmap))) x) \/
           PS.In x FVset)) /\
       (forall B Scope FVset,
-         let '(Scope', FVset') := fundefs_true_fv_aux funmap B Scope FVset in
+         let '(Scope', FVset') := fundefs_true_fv_aux lift_dec funmap B Scope FVset in
          (forall x, PS.In x Scope' <-> (PS.In x Scope \/ In _ (name_in_fundefs B) x)) /\
          (forall x, PS.In x FVset' ->
                ((In _ (occurs_free_fundefs B) x /\ ~ PS.In x Scope) \/
@@ -453,7 +664,38 @@ Section Lambda_lifting_corresp.
         + destruct (PS.mem v0 Scope) eqn:Heq; eauto. inv H0; eauto.
           apply_set_specs_ctx; eauto. left; split; eauto.
           intros Hc.  apply PS.mem_spec in Hc. congruence.
-      - destruct (fundefs_true_fv_aux funmap f2 Scope FVset) as [Scope' FVset'] eqn:Heq.
+      - eapply IHe in H. inv H.
+        + inv H0. left. split. eapply Free_Eletapp2; eauto.
+          intros Hc. subst. apply H1. now apply_set_specs; eauto.
+          intros Hc. apply H1. now apply_set_specs; eauto.
+        + inv H0; eauto. eapply add_list_spec in H. inv H. 
+          * destruct (funmap ! f) eqn:Hget.
+            -- destruct f0; eauto. destruct (lift_dec l0 FVset).
+                ++ eapply union_list_spec in H0. inv H0.
+                   ** repeat apply_set_specs_ctx; eauto.
+                      right. left. right. eexists.
+                      split. eexists. erewrite lifted_name_eq; eauto.
+                      unfold fun_map. simpl.
+                      rewrite Hget. reflexivity.
+                      unfold lifted_name, fun_map. simpl.
+                      rewrite Hget. reflexivity.
+                   ** right. left. left. do 4 eexists.
+                      unfold fun_map. rewrite Hget. eauto.
+                ++ destruct (PS.mem f Scope) eqn:Heq; eauto.
+                   repeat apply_set_specs_ctx; eauto.
+                   left. constructor. constructor; eauto. now left.
+                   intros Hc. eapply PS.mem_spec in Hc. congruence.
+                ++ destruct (PS.mem f Scope) eqn:Heq; eauto.
+                   repeat apply_set_specs_ctx; eauto.
+                   left. constructor. constructor; eauto. now left.
+                   intros Hc. eapply PS.mem_spec in Hc. congruence.
+            -- destruct (PS.mem f Scope) eqn:Heq; eauto.
+               repeat apply_set_specs_ctx; eauto.
+               left. constructor. constructor; eauto. now left.
+               intros Hc. eapply PS.mem_spec in Hc. congruence.
+          * destructAll.                   
+            left. constructor. constructor; eauto. now right. eassumption.                  
+      - destruct (fundefs_true_fv_aux lift_dec funmap f2 Scope FVset) as [Scope' FVset'] eqn:Heq.
         specialize (IHdefs Scope FVset). rewrite Heq in IHdefs.
         destruct IHdefs as [H1 H2].
         eapply IHe in H. inv H.
@@ -461,25 +703,31 @@ Section Lambda_lifting_corresp.
           intros Hc. eapply H3. eapply H1; eauto.
           intros Hc. eapply H3. eapply H1; eauto.
         + inv H0; eauto. eapply H2 in H. inv H; eauto. inv H0; eauto.
-      - destruct (Maps.PTree.get v funmap) eqn:Heqf.
-        + destruct f. eapply add_list_spec in H. inv H; eauto.
-          repeat apply_set_specs_ctx; eauto.
-          right; left; right. repeat eexists. erewrite lifted_name_eq; eauto.
-          unfold fun_map. rewrite Heqf; reflexivity.
-          erewrite lifted_name_eq; eauto.
-          unfold fun_map. rewrite Heqf; reflexivity.
-          right; left; left. repeat eexists.
-          unfold fun_map. rewrite Heqf; reflexivity.
-          eassumption.
-          now inv H0; left; split; eauto.
-        + destruct (PS.mem v Scope) eqn:Heq; eauto.
-          * eapply add_list_spec in H. inv H; eauto.
-            inv H0. left. split; eauto.
-          * eapply add_list_spec in H. inv H; eauto.
+      - eapply add_list_spec in H. inv H; eauto.
+        + destruct (Maps.PTree.get v funmap) eqn:Heqf.
+          destruct f. destruct (lift_dec l1 FVset); eauto. 
+          * repeat apply_set_specs_ctx; eauto.
+            right; left; right. repeat eexists. erewrite lifted_name_eq; eauto.
+            unfold fun_map. rewrite Heqf; reflexivity.
+            erewrite lifted_name_eq; eauto.
+            unfold fun_map. rewrite Heqf; reflexivity.
+            right; left; left. repeat eexists.
+            unfold fun_map. rewrite Heqf; reflexivity.
+            eassumption.
+          * destruct (PS.mem v Scope) eqn:Heq; eauto.
             repeat apply_set_specs_ctx; eauto.
             left; split; eauto. intros Hc.
             eapply PS.mem_spec in Hc. congruence.
-            inv H0; eauto.
+          * destruct (PS.mem v Scope) eqn:Heq; eauto.
+            repeat apply_set_specs_ctx; eauto.
+            left. split; eauto. intros Hc.
+            eapply PS.mem_spec in Hc. congruence.
+          * destruct (PS.mem v Scope) eqn:Heq; eauto.
+            repeat apply_set_specs_ctx; eauto.
+            left. split; eauto. intros Hc.
+            eapply PS.mem_spec in Hc. congruence.
+        + destructAll.
+          repeat apply_set_specs_ctx; eauto.
       - eapply IHe in H. inv H.
         + inv H0. left. split. eapply Free_Eprim2 ; eauto.
           intros Hc. subst. apply H1. now apply_set_specs; eauto.
@@ -489,7 +737,7 @@ Section Lambda_lifting_corresp.
       - destruct (PS.mem v Scope) eqn:Heq; eauto.
         repeat apply_set_specs_ctx; eauto. left; split; eauto.
         intros Hc. eapply PS.mem_spec in Hc. congruence.
-      - destruct (fundefs_true_fv_aux funmap f5 (PS.add v Scope) FVset) as [Scope' FVset'] eqn:Heq.
+      - destruct (fundefs_true_fv_aux lift_dec funmap f5 (PS.add v Scope) FVset) as [Scope' FVset'] eqn:Heq.
         specialize (IHdefs (PS.add v Scope) FVset). rewrite Heq in IHdefs.
         destruct IHdefs as [H1 H2]. split. 
         + split; intros H.
@@ -514,14 +762,14 @@ Section Lambda_lifting_corresp.
         intros x. intros H; eauto.
     Qed.
 
-    Corollary fundefs_true_fv_correct B :
-      Included var (FromList (PS.elements (fundefs_true_fv funmap B)))
+    Corollary fundefs_true_fv_correct B lift_dec :
+      Included var (FromList (PS.elements (fundefs_true_fv lift_dec funmap B)))
                (Union _ (occurs_free_fundefs B)
                       (Union _ (FunsFVs (fun_map funmap)) (LiftedFuns (fun_map funmap)))).
     Proof.
-      destruct exp_true_fv_fundefs_true_fv_correct as [_ H2].
+      destruct (exp_true_fv_fundefs_true_fv_correct lift_dec) as [_ H2].
       unfold fundefs_true_fv. specialize (H2 B PS.empty PS.empty).
-      destruct (fundefs_true_fv_aux funmap B PS.empty PS.empty) as [scope fvs].
+      destruct (fundefs_true_fv_aux lift_dec funmap B PS.empty PS.empty) as [scope fvs].
       intros x H. inv H2.
       assert (Hin : PS.In x fvs).
       { eapply PS.elements_spec1. eapply InA_alt.
@@ -534,33 +782,45 @@ Section Lambda_lifting_corresp.
   End TrueFV_correct.
   
   (** * The lambda lifting algorithm is sound w.r.t. its relational specification *)
-  Lemma lambda_lifting_sound :
-    (forall (e : exp) (FVmap : VarInfoMap) (FNmap : FunInfoMap) (S : Ensemble var)
+  Lemma lambda_lifting_sound max_args max_push lift_dec :
+    (forall (e : exp) (FVmap : VarInfoMap) (FNmap : FunInfoMap) (GFuns: GFunMap)
+            (Scope AFuns : PS.t) (S : Ensemble var)
        (Hlf : Disjoint _ (LiftedFuns (fun_map FNmap)) (Union _ S (bound_var e)))
        (Hfvs : Disjoint _ (FunsFVs (fun_map FNmap)) (Union _ S (bound_var e)))
        (Hf : Disjoint _ S (Union _ (bound_var e) (occurs_free e)))
        (HD : Disjoint _ (bound_var e) (occurs_free e))
-       (Hnin : binding_not_in_map (Union _ S (bound_var e)) FVmap)
+       (Hnin : Disjoint _  (Union _ S (bound_var e)) (Dom_map FVmap))
+       (Hnin' : Disjoint _  (bound_var e) (Dom_map FNmap))
+       
        (Hun : unique_bindings e),
-       {{ fun s => fresh S (next_var s) }}
-         exp_lambda_lift e FVmap FNmap
-       {{ fun s e' s' =>
+       {{ fun r s => fresh S (next_var (fst s)) }}
+         exp_lambda_lift max_args max_push lift_dec e Scope AFuns FVmap FNmap GFuns
+       {{ fun r s e' s' =>
            exists S', Exp_lambda_lift (fun_map FNmap) (rename FVmap) e S e' S' /\
-                 fresh S' (next_var s')
+                      fresh S' (next_var (fst s'))
         }}) /\
-    (forall (B : fundefs) (FVmap : VarInfoMap) (FNmap : FunInfoMap) (S : Ensemble var)
+    (forall (B B0 : fundefs) (FVmap : VarInfoMap) (FNmap : FunInfoMap) (GFuns: GFunMap)
+            (names AFuns : PS.t) (S : Ensemble var) (no : nat)
        (Hlf : Disjoint _ (LiftedFuns (fun_map FNmap)) (Union _ S (bound_var_fundefs B)))
        (Hfvs : Disjoint _ (FunsFVs (fun_map FNmap)) (Union _ S (bound_var_fundefs B)))
-       (Hf : Disjoint _ S (Union _ (bound_var_fundefs B) (occurs_free_fundefs B)))
+       (Hf : Disjoint _ S ((bound_var_fundefs B :|: occurs_free_fundefs B) :|: bound_var_fundefs B0))
+       (Hdis : Disjoint _ (bound_var_fundefs B \\ name_in_fundefs B) (name_in_fundefs B0))
        (HD : Disjoint _ (bound_var_fundefs B) (occurs_free_fundefs B))
-       (Hin1 : Included _ (name_in_fundefs B) (domain (fun_map FNmap)))
-       (Hnin : binding_not_in_map (Union _ S (bound_var_fundefs B)) FVmap)
-       (Hun : unique_bindings_fundefs B),
-       {{ fun s => fresh S (next_var s) }}
-         fundefs_lambda_lift B FVmap FNmap
-       {{ fun s B' s' =>     
-            exists S', Fundefs_lambda_lift (fun_map FNmap) (rename FVmap) B S B' S' /\
-            fresh S' (next_var s')
+       (Hnin : Disjoint _  (Union _ S (bound_var_fundefs B :|: bound_var_fundefs B0)) (Dom_map FVmap))
+       (Hnin' : Disjoint _  (bound_var_fundefs B \\ name_in_fundefs B) (Dom_map FNmap))
+       (Hun : unique_bindings_fundefs B)
+       (Hor : (name_in_fundefs B \subset domain (fun_map FNmap) /\ name_in_fundefs B0 \subset domain (fun_map FNmap)) \/ 
+              (Disjoint _ (name_in_fundefs B) (domain (fun_map FNmap)) /\ Disjoint _ (name_in_fundefs B0) (domain (fun_map FNmap))  ))
+       (Hdom : name_in_fundefs B \subset Dom_map FNmap),
+       {{ fun r s => fresh S (next_var (fst s)) }}
+         fundefs_lambda_lift max_args max_push lift_dec B B0 names AFuns FVmap FNmap GFuns no
+         {{ fun r s B' s' =>     
+              exists S',
+                (name_in_fundefs B \subset domain (fun_map FNmap) ->
+                 Fundefs_lambda_lift2 (fun_map FNmap) (rename FVmap) B0 B S B' S') /\
+                (Disjoint _ (name_in_fundefs B) (domain (fun_map FNmap)) ->
+                 Fundefs_lambda_lift3 (fun_map FNmap) (rename FVmap) B0 B S B' S') /\
+                fresh S' (next_var (fst s'))
         }}).
   Proof with now eauto with Ensembles_DB functions_BD.
     exp_defs_induction IHe IHl IHB; simpl; intros.
@@ -573,14 +833,11 @@ Section Lambda_lifting_corresp.
         * eapply Disjoint_Included_r. now apply occurs_free_Econstr_Included.
           eapply Union_Disjoint_r. now eauto with Ensembles_DB.
           eapply Disjoint_Singleton_r; eassumption.
-        * eapply binding_not_in_map_antimon; [| eassumption ].
-          normalize_bound_var...
-      + intros x s1. apply return_triple.
-        intros s2 [S' [Hexp Hfr]]. eexists; split; eauto.
+      + intros x s1. apply return_triple. 
+        intros _ [c2 _u] [S' [Hexp Hfr]]. eexists; split; eauto.
         constructor; eauto. rewrite <- rename_not_in_domain_f_eq.
         eassumption.
-        eapply binding_not_in_map_antimon; [| eassumption ].
-        normalize_bound_var...
+        repeat normalize_bound_var_in_ctx. eapply Disjoint_In_l. eassumption. sets.
     - eapply return_triple. intros s Hfr.
       eexists. split; eauto. constructor.
     - setoid_rewrite assoc. eapply bind_triple.
@@ -591,8 +848,6 @@ Section Lambda_lifting_corresp.
         * eapply Disjoint_Included; [| | now apply HD ].
           normalize_occurs_free...
           now eauto with Ensembles_DB.
-        * eapply binding_not_in_map_antimon; [| eassumption ].
-          normalize_bound_var...
       + intros e' s1. simpl. 
         setoid_rewrite st_eq_Ecase. eapply pre_existential.
         intros S1. eapply pre_curry_l; intros Hll.
@@ -612,10 +867,9 @@ Section Lambda_lifting_corresp.
             - eapply Disjoint_Included; [| | now apply HD ].
               normalize_occurs_free...
               now eauto with Ensembles_DB.
-            - eapply binding_not_in_map_antimon; [| eassumption ].
-              eapply Included_Union_compat.
-              now eapply Exp_Lambda_lift_free_set_Included; eauto.
-              normalize_bound_var...
+            - eapply Exp_Lambda_lift_free_set_Included in Hll. 
+              sets.
+            - sets.
             - inv Hun; eauto. }
         * intros e1 s2. eapply pre_existential.
           intros S2. eapply pre_curry_l; intros Hll'.
@@ -631,153 +885,309 @@ Section Lambda_lifting_corresp.
         * eapply Disjoint_Included_r. now apply occurs_free_Eproj_Included.
           eapply Union_Disjoint_r. now eauto with Ensembles_DB.
           eapply Disjoint_Singleton_r; eassumption.
-        * eapply binding_not_in_map_antimon; [| eassumption ].
-          normalize_bound_var...
       + intros x s1. apply return_triple.
-        intros s2 [S' [Hexp Hfr]]. eexists; split; eauto.
+        intros _ [c2 _u] [S' [Hexp Hfr]]. eexists; split; eauto.
         constructor; eauto. rewrite <- rename_not_in_domain_f_eq.
         eassumption.
-        eapply binding_not_in_map_antimon; [| eassumption ].
-        normalize_bound_var...
-    - assert (HFV : Included var (FromList (PS.elements (fundefs_true_fv FNmap f2)))
+        repeat normalize_bound_var_in_ctx. eapply Disjoint_In_l. eassumption. sets.
+    - eapply bind_triple.
+      + inv Hun. repeat normalize_bound_var_in_ctx. eapply IHe; try eauto with Ensembles_DB.
+        * eapply Disjoint_Included_r; [| eassumption ].
+          rewrite <- bound_var_Eletapp.
+          now apply bound_var_occurs_free_Eletapp_Included.
+        * eapply Disjoint_Included_r. now apply occurs_free_Eletapp_Included.
+          eapply Union_Disjoint_r. now eauto with Ensembles_DB.
+          eapply Disjoint_Singleton_r; eassumption.
+      + intros z s1. simpl. destruct (FNmap ! f) eqn:Hget.
+        destruct f0. destruct (lift_dec l0 Scope).
+        * apply return_triple. 
+          intros _ [c2 _u] [S' [Hexp Hfr]]. eexists; split; eauto.
+          constructor; eauto. unfold fun_map. rewrite Hget. reflexivity. rewrite <- rename_not_in_domain_f_eq.
+          eassumption.
+          repeat normalize_bound_var_in_ctx. eapply Disjoint_In_l. eassumption. sets.
+        * apply return_triple. 
+          intros _ [c2 _u] [S' [Hexp Hfr]]. eexists; split; eauto.
+          eapply LL_Eletapp_unknown.
+          rewrite <- rename_not_in_domain_f_eq.
+          eassumption.
+          repeat normalize_bound_var_in_ctx. eapply Disjoint_In_l. eassumption. sets.
+        * apply return_triple. 
+          intros _ [c2 _u] [S' [Hexp Hfr]]. eexists; split; eauto.
+          eapply LL_Eletapp_unknown.
+          rewrite <- rename_not_in_domain_f_eq.
+          eassumption.
+          repeat normalize_bound_var_in_ctx. eapply Disjoint_In_l. eassumption. sets.
+        * apply return_triple. 
+          intros _ [c2 _u] [S' [Hexp Hfr]]. eexists; split; eauto.
+          eapply LL_Eletapp_unknown.
+          rewrite <- rename_not_in_domain_f_eq.
+          eassumption.
+          repeat normalize_bound_var_in_ctx. eapply Disjoint_In_l. eassumption. sets.
+    - assert (HFV : Included var (FromList (PS.elements (fundefs_true_fv lift_dec FNmap f2)))
                              (Union var (occurs_free_fundefs f2)
                                     (Union var (FunsFVs (fun_map FNmap)) (LiftedFuns (fun_map FNmap)))))
         by eapply fundefs_true_fv_correct.
-      eapply bind_triple.
-      + eapply add_functions_sound.
-        eapply binding_not_in_map_antimon; [| eassumption ].
-        normalize_bound_var...
-      + intros m s1. eapply pre_existential. intros σ'.
-        eapply pre_existential. intros ζ'. eapply pre_existential. intros S1.
-        eapply pre_curry_l. intros Hadd. eapply pre_curry_l. intros Heq1.
-        eapply pre_curry_l. intros Heq2.
-        eapply bind_triple.
-        * { inv Hun . eapply IHB; eauto.
-            - rewrite <- Heq2. eapply Disjoint_Included_l. 
-              eapply Add_functions_LiftedFuns_Included_r. eassumption.
-              eapply Union_Disjoint_l.
-              eapply Disjoint_Included_r; [| eassumption ].
-              eapply Included_Union_compat.
-              now eapply Add_functions_free_set_Included; eauto.
-              normalize_bound_var...
-              eapply Union_Disjoint_r. now eauto with Ensembles_DB.
-              eapply Disjoint_Included; [| | now apply Hf ].
-              normalize_bound_var... now eauto with Ensembles_DB.
-            - rewrite <- Heq2. eapply Disjoint_Included_l.
-              eapply Add_functions_FunsFVs_Included_r. eassumption.
-              eapply Union_Disjoint_l.
-              eapply Disjoint_Included_r; [| eassumption ].
-              eapply Included_Union_compat.
-              now eapply Add_functions_free_set_Included; eauto.
-              normalize_bound_var...
-              eapply Disjoint_Included_l; [ eassumption |].
-              eapply Union_Disjoint_l.
-              eapply Disjoint_sym. eapply Union_Disjoint_l. 
-              eapply Disjoint_Included; [| | now apply Hf ].
-              normalize_occurs_free...
-              now eapply Add_functions_free_set_Included; eauto.
-              eapply Disjoint_Included; [| | now apply HD ].
-              normalize_occurs_free... normalize_bound_var...
-              eapply Union_Disjoint_l.
-              eapply Disjoint_Included_r; [| eassumption ].
-              eapply Included_Union_compat.
-              now eapply Add_functions_free_set_Included; eauto.
-              normalize_bound_var...
-              eapply Disjoint_Included_r; [| eassumption ].
-              eapply Included_Union_compat.
-              now eapply Add_functions_free_set_Included; eauto.
-              normalize_bound_var...
-            - eapply Disjoint_Included; [| | now apply Hf].
-              normalize_bound_var. normalize_occurs_free...
-              now eapply Add_functions_free_set_Included; eauto.
-            - eapply Disjoint_Included; [| | now apply HD].
-              normalize_occurs_free...
-              normalize_bound_var...
-            - rewrite <- Heq2, <- Funs_Same_set at 1.
-              rewrite Add_functions_Funs_Same_set; eauto...
-            - eapply binding_not_in_map_antimon; [| eassumption ].
-              eapply Included_Union_compat.
-              now eapply Add_functions_free_set_Included; eauto.
-              normalize_bound_var... }
-        * intros B' s2. eapply pre_existential. intros S2.
-          eapply pre_curry_l. intros Hll.
+      set (fvs := (PS.filter
+                      (fun x : PS.elt =>
+                         match GFuns ! x with
+                         | Some _ => false
+                         | None => true
+                         end) (fundefs_true_fv lift_dec FNmap f2))).
+
+      set (args := (if
+                       max_args - fundefs_max_params f2 <?
+                       Datatypes.length
+                         (if
+                             existsb (fun x : var => max_push <? stack_push_fundefs x f2)
+                                     (PS.elements fvs)
+                           then []
+                           else PS.elements fvs)
+                     then []
+                     else
+                       if
+                         existsb (fun x : var => max_push <? stack_push_fundefs x f2) (PS.elements fvs)
+                       then []
+                       else PS.elements fvs)).
+
+      assert (Hsub : FromList args \subset FromList (PS.elements (fundefs_true_fv lift_dec FNmap f2))).
+      { unfold args.
+        destruct (_ <? _). normalize_sets. now sets.
+        destruct (existsb _). normalize_sets. now sets.
+        unfold fvs. rewrite <- !FromSet_elements.
+        intros s Hin. eapply FromSet_sound in Hin; [| reflexivity ].
+        eapply PS.filter_spec in Hin. destructAll. eapply FromSet_complete. reflexivity. eassumption.
+        clear. intro; intros. subst. reflexivity. }
+      assert (Hndargs : NoDup args).
+      { unfold args.
+        destruct (_ <? _). now constructor.
+        destruct (existsb _). now constructor.
+        unfold fvs.
+        eapply NoDupA_NoDup. eapply PS.elements_spec2w. }
+
+      destruct (Datatypes.length (PS.elements fvs) =? Datatypes.length args)%nat eqn:Heqb.
+      { eapply bind_triple.
+        + eapply add_functions_true_sound; eauto.
+          repeat normalize_bound_var_in_ctx.
+          eapply Disjoint_Included_l; [| eassumption ]. sets.
+        + intros [m gm] [s1 _u]. eapply pre_existential. intros σ'.
+          eapply pre_existential. intros ζ'. eapply pre_existential. intros S1.
+          eapply pre_curry_l. intros Hadd. eapply pre_curry_l. intros Hsub'.
+          eapply pre_curry_l. intros Hdom.
+          eapply pre_curry_l. intros Heq1. eapply pre_curry_l. intros Heq2. 
           eapply bind_triple.
-          { inv Hun. repeat normalize_bound_var_in_ctx. eapply IHe; eauto.
-            - rewrite <- Heq2. eapply Disjoint_Included_l. 
-              eapply Add_functions_LiftedFuns_Included_r. eassumption.
-              eapply Union_Disjoint_l.
-              eapply Disjoint_Included_r; [| eassumption ].
-              eapply Included_Union_compat.
-              eapply Included_trans.
-              now eapply Fundefs_Lambda_lift_free_set_Included; eauto.
-              now eapply Add_functions_free_set_Included; eauto.
-              now eauto with Ensembles_DB.
-              eapply Union_Disjoint_r.
-              eapply Disjoint_Included_r.
-              now eapply Fundefs_Lambda_lift_free_set_Included; eauto.
-              now eauto with Ensembles_DB.
-              eapply Disjoint_Included; [| | now apply Hf ]...
-            - rewrite <- Heq2. eapply Disjoint_Included_l.
-              eapply Add_functions_FunsFVs_Included_r. eassumption.
-              eapply Union_Disjoint_l.
-              eapply Disjoint_Included_r; [| eassumption ].
-              eapply Included_Union_compat. eapply Included_trans.              
-              now eapply Fundefs_Lambda_lift_free_set_Included; eauto.
-              now eapply Add_functions_free_set_Included; eauto.
-              now eauto with Ensembles_DB.
-              eapply Disjoint_Included_l; [ eassumption |].
-              eapply Union_Disjoint_l.
-              eapply Disjoint_sym. eapply Union_Disjoint_l. 
-              eapply Disjoint_Included; [| | now apply Hf ].
-              normalize_occurs_free...
-              eapply Included_trans.
-              now eapply Fundefs_Lambda_lift_free_set_Included; eauto.
-              now eapply Add_functions_free_set_Included; eauto.
-              eapply Disjoint_Included; [| | now apply HD ].
-              normalize_occurs_free... now eauto with Ensembles_DB.
-              eapply Union_Disjoint_l.
-              eapply Disjoint_Included_r; [| eassumption ].
-              eapply Included_Union_compat.
-              eapply Included_trans.
-              now eapply Fundefs_Lambda_lift_free_set_Included; eauto. 
-              now eapply Add_functions_free_set_Included; eauto.
-              now eauto with Ensembles_DB.
-              eapply Disjoint_Included_r; [| eassumption ].
-              eapply Included_Union_compat.
-              eapply Included_trans.
-              now eapply Fundefs_Lambda_lift_free_set_Included; eauto.
-              now eapply Add_functions_free_set_Included; eauto.
-              now eauto with Ensembles_DB.
-            - eapply Disjoint_Included; [| | now apply Hf].
-              eapply Union_Included. now eauto with Ensembles_DB.
-              eapply Included_trans. now eapply occurs_free_Efun_Included.
-              eapply Union_Included. now eauto with Ensembles_DB.
-              eapply Included_trans. now apply name_in_fundefs_bound_var_fundefs.
-              now eauto with Ensembles_DB.
-              eapply Included_trans. now eapply Fundefs_Lambda_lift_free_set_Included; eauto.
-              now eapply Add_functions_free_set_Included; eauto.
-            - eapply Disjoint_Included_r.
-              now apply occurs_free_Efun_Included.
-              eapply Union_Disjoint_r. now eauto with Ensembles_DB.
-              eapply Disjoint_Included_r. now apply name_in_fundefs_bound_var_fundefs. 
-              assumption.
-            - eapply binding_not_in_map_antimon; [| eassumption ].
-              eapply Included_Union_compat.
-              eapply Included_trans.
-              now eapply Fundefs_Lambda_lift_free_set_Included; eauto.
-              now eapply Add_functions_free_set_Included; eauto.
-              normalize_bound_var... }
-          intros e' s3. eapply return_triple. intros s4 [S3 [Hll' Hfr]].
-          eexists; split; eauto. rewrite <- Heq1, <- Heq2 in Hll, Hll'. 
-          econstructor; [| | eassumption | eassumption | eassumption ].
-          eassumption.
-          eapply NoDupA_NoDup. now eapply PS.elements_spec2w.
-    - edestruct (M.get v FNmap) as [ [ ? ? ? ] | ] eqn:Heq;
-      eapply return_triple; intros s1 Hfr.
-      + eexists. split; eauto.
+          * { inv Hun. eapply IHB; eauto.
+              - rewrite <- Heq2. eapply Disjoint_Included_l. 
+                eapply Add_functions_LiftedFuns_Included_r. eassumption.
+                eapply Union_Disjoint_l.
+                eapply Disjoint_Included_r; [| eassumption ].
+                eapply Included_Union_compat.
+                now eapply Add_functions_free_set_Included; eauto.
+                normalize_bound_var...
+                eapply Union_Disjoint_r. now eauto with Ensembles_DB.
+                eapply Disjoint_Included; [| | now apply Hf ].
+                normalize_bound_var... now eauto with Ensembles_DB.
+              - rewrite <- Heq2. eapply Disjoint_Included_l.
+                eapply Add_functions_FunsFVs_Included_r. eassumption.
+                eapply Union_Disjoint_l.
+                eapply Disjoint_Included_r; [| eassumption ].
+                eapply Included_Union_compat.
+                now eapply Add_functions_free_set_Included; eauto.
+                normalize_bound_var...
+                repeat sets. 
+                eapply Disjoint_Included_l; [ eassumption |].
+                eapply Disjoint_Included_l; [ eassumption |].                
+                eapply Union_Disjoint_l.
+                eapply Disjoint_sym. eapply Union_Disjoint_l. 
+                eapply Disjoint_Included; [| | now apply Hf ].
+                normalize_occurs_free...
+                now eapply Add_functions_free_set_Included; eauto.
+                eapply Disjoint_Included; [| | now apply HD ].
+                normalize_occurs_free... normalize_bound_var...
+                eapply Union_Disjoint_l.
+                eapply Disjoint_Included_r; [| eassumption ].
+                eapply Included_Union_compat.
+                now eapply Add_functions_free_set_Included; eauto.
+                normalize_bound_var...
+                eapply Disjoint_Included_r; [| eassumption ].
+                eapply Included_Union_compat.
+                now eapply Add_functions_free_set_Included; eauto.
+                normalize_bound_var...
+              - eapply Disjoint_Included; [| | now apply Hf].
+                normalize_bound_var. normalize_occurs_free...
+                now eapply Add_functions_free_set_Included; eauto.
+              - now sets.
+              - eapply Disjoint_Included; [| | now apply HD].
+                normalize_occurs_free...
+                normalize_bound_var...
+              - eapply Disjoint_Included_l; [| eassumption ].
+                normalize_bound_var. eapply Add_functions_free_set_Included in Hadd.
+                sets.
+              - rewrite Hdom. repeat normalize_bound_var_in_ctx.
+                eapply Union_Disjoint_r. now sets.
+                sets.
+              - rewrite Hdom. sets. }
+          * intros B' s2. eapply pre_existential. intros S2.
+            eapply pre_curry_l. intros Hll.
+            eapply pre_curry_l. intros HDis.
+            eapply bind_triple.
+            { eapply make_wrappers_sound_subset. eassumption. }
+            { intros [Bw m'] [c u]. inv Hun. repeat normalize_bound_var_in_ctx.
+              eapply pre_existential. intros Bw'.
+              eapply pre_existential. intros sig.
+              eapply pre_existential. intros S'.
+              eapply pre_curry_l. intros Hbw. subst.
+              eapply pre_curry_l. intros Hw.
+              eapply pre_curry_l. intros Hfeq.
+              eapply pre_curry_l. intros Hdom'.
+              eapply bind_triple.
+              assert (Hfs : S' \subset S). 
+              { eapply Included_trans.
+                now eapply Make_wrappers_free_set_Included; eauto. eapply Included_trans. 
+                now eapply Fundefs_Lambda_lift_free_set_Included2; eauto.                
+                now eapply Add_functions_free_set_Included; eauto. }
+
+              eapply IHe; eauto.
+              - rewrite <- Heq2. eapply Disjoint_Included_l. 
+                eapply Add_functions_LiftedFuns_Included_r. eassumption.
+                eapply Union_Disjoint_l.
+                eapply Disjoint_Included_r; [| eassumption ].
+                eapply Included_Union_compat. eassumption.
+                now sets.
+                eapply Union_Disjoint_r.
+                eapply Disjoint_Included_r. 
+                now eapply Make_wrappers_free_set_Included; eauto.
+                eapply Disjoint_Included_r.
+                now eapply Fundefs_Lambda_lift_free_set_Included2; eauto.                
+                now sets. sets.
+              - rewrite <- Heq2. eapply Disjoint_Included_l.
+                eapply Add_functions_FunsFVs_Included_r. eassumption.
+                eapply Union_Disjoint_l.
+                eapply Disjoint_Included_r; [| eassumption ]. 
+                eapply Included_Union_compat. eassumption.
+                now eauto with Ensembles_DB.
+                eapply Disjoint_Included_l; [ eassumption |].
+                eapply Disjoint_Included_l; [ eassumption |].
+                repeat normalize_occurs_free_in_ctx. 
+                eapply Union_Disjoint_l; sets.
+                + eapply Union_Disjoint_r; sets.
+                  eapply Disjoint_sym. eapply Disjoint_Included; [| | eapply Hf ]. now sets.
+                  eassumption.
+                  eapply Disjoint_sym. eapply Disjoint_Included; [| | eapply HD]; sets.
+                + eapply Union_Disjoint_l; sets.
+              - eapply Disjoint_Included; [| | now apply Hf].
+                eapply Union_Included. now eauto with Ensembles_DB.
+                eapply Included_trans. now eapply occurs_free_Efun_Included.
+                eapply Union_Included. now eauto with Ensembles_DB.
+                eapply Included_trans. now apply name_in_fundefs_bound_var_fundefs.
+                now eauto with Ensembles_DB. eassumption.
+              - eapply Disjoint_Included_r.
+                now apply occurs_free_Efun_Included.
+                eapply Union_Disjoint_r. now eauto with Ensembles_DB.
+                eapply Disjoint_Included_r. now apply name_in_fundefs_bound_var_fundefs. 
+                assumption.
+              - rewrite Hdom'. eapply Union_Disjoint_r; sets.
+                eapply Disjoint_Included_r. eapply name_in_fundefs_bound_var_fundefs.
+                eapply Union_Disjoint_l; eauto.
+                eapply Disjoint_Included; [| | eapply Hf ]; sets.
+              - rewrite Hdom. eapply Union_Disjoint_r; sets.
+                eapply Disjoint_Included_r. now apply name_in_fundefs_bound_var_fundefs.
+                eassumption.
+              - intros e' s3. eapply return_triple. intros _ s4 [S3 [Hll' Hfr]].
+                eexists; split.
+                edestruct Make_wrappers_f_eq. eassumption. symmetry. eassumption. symmetry. eassumption.
+                destructAll.
+                
+                eapply LL_Efun2; [ | | | | eapply H | ]. 5:{ rewrite <- H0, <- Hfeq, Heq2. eassumption. } 
+                4:{ rewrite Heq2, Heq1. eapply Hll. eassumption. }
+                3:{ eassumption. }
+                eapply Included_trans. eassumption.
+                eapply Included_trans. eassumption.
+                
+                edestruct Add_functions_f_eq. eassumption. symmetry. eassumption. reflexivity.
+                reflexivity.  reflexivity. eassumption. eassumption. } }
+      { inv Hun. eapply bind_triple.
+        + eapply add_functions_false_sound; eauto.
+          repeat normalize_bound_var_in_ctx.
+          eapply Disjoint_Included_l; [| eassumption ]. sets.
+        + intros [m gm] [s1 _u]. 
+          eapply pre_curry_l. intros Hdom.
+          eapply pre_curry_l. intros Heq1. eapply pre_curry_l. intros Heq2. 
+          eapply bind_triple.
+          * { repeat normalize_bound_var_in_ctx. repeat normalize_occurs_free_in_ctx. 
+              eapply IHB; eauto.
+              - rewrite <- Heq2. eapply Disjoint_Included_l. reflexivity.
+                 now sets.
+              - rewrite <- Heq2. now sets. 
+              - now sets.
+              - now sets.
+              - eapply Disjoint_Included; [| | now apply HD]; sets.                
+              - now sets.
+              - rewrite Hdom. now sets.
+              - rewrite Hdom. now sets. } 
+          * intros B' s2. eapply pre_existential. intros S2.
+            eapply pre_curry_l. intros Hll.
+            eapply pre_curry_l. intros HDis.
+            eapply bind_triple.
+            { eapply make_wrappers_sound_Disjoint.
+              - intro. subst. simpl in *. repeat normalize_sets. congruence.
+              - rewrite Hdom. sets.
+              - eassumption. }
+            { intros [Bw m'] [c u]. 
+              eapply pre_curry_l. intro; subst. 
+              eapply pre_curry_l. intro; subst. 
+              eapply bind_triple.
+              repeat normalize_bound_var_in_ctx.
+              repeat normalize_occurs_free_in_ctx.
+              eapply IHe; eauto.
+              - rewrite <- Heq2.
+                eapply Union_Disjoint_r.
+                eapply Disjoint_Included_r. 
+                eapply Fundefs_Lambda_lift_free_set_Included3; eauto.                
+                now sets. now sets.
+              - rewrite <- Heq2.
+                eapply Union_Disjoint_r.
+                eapply Disjoint_Included_r. 
+                eapply Fundefs_Lambda_lift_free_set_Included3; eauto.                
+                now sets. now sets.
+              - eapply Disjoint_Included; [| | now apply Hf].
+                rewrite !Union_assoc. rewrite Union_Setminus_Included. 
+                now sets. tci. eapply Included_trans. eapply name_in_fundefs_bound_var_fundefs. now sets.
+                eapply Fundefs_Lambda_lift_free_set_Included3; eauto.                
+              - eapply Disjoint_Included_r. eapply Included_Union_Setminus with (s4 := name_in_fundefs f2).
+                tci.
+                eapply Union_Disjoint_r.
+                eapply Disjoint_Included; [| | eapply HD ]; now sets.
+                eapply Disjoint_Included_r; [| eassumption ].
+                eapply name_in_fundefs_bound_var_fundefs.
+              - eapply Union_Disjoint_l.
+                eapply Disjoint_Included_l. 
+                eapply Fundefs_Lambda_lift_free_set_Included3; eauto.                
+                now sets. now sets.
+              - rewrite Hdom. eapply Union_Disjoint_r; sets.
+                eapply Disjoint_Included_r. eapply name_in_fundefs_bound_var_fundefs.
+                eassumption. 
+              - intros e' s3. eapply return_triple. intros _ s4 [S3 [Hll' Hfr]].                
+                eexists; split.  eapply LL_Efun3.
+                rewrite Heq2. now eauto.
+                rewrite <- rename_not_in_domain_add_extend_fundefs_f_eq. rewrite Heq2. eassumption.
+                eapply Disjoint_Included_l. eapply name_in_fundefs_bound_var_fundefs.
+                repeat normalize_bound_var_in_ctx. now sets.
+                eassumption. } }
+    - edestruct (M.get v FNmap) as [ [ | ] | ] eqn:Heq.
+      destruct (lift_dec l1 Scope).
+      + eapply return_triple; intros u s1 Hfr.
+        eexists. split; eauto.
         econstructor. unfold fun_map. rewrite Heq. reflexivity.
-      + eexists. split; eauto. econstructor. 
-    - eapply bind_triple.
+      + eapply return_triple; intros u s1 Hfr.
+        eexists. split; eauto.
+        econstructor.
+      + eapply return_triple; intros u s1 Hfr.
+        eexists. split; eauto.
+        econstructor.
+      + eapply return_triple; intros u s1 Hfr.
+        eexists. split; eauto.
+        econstructor.
+    - simpl. eapply bind_triple.
       + inv Hun. repeat normalize_bound_var_in_ctx. eapply IHe; try eauto with Ensembles_DB.
         * eapply Disjoint_Included_r; [| eassumption ].
           rewrite <- bound_var_Eprim.
@@ -785,98 +1195,191 @@ Section Lambda_lifting_corresp.
         * eapply Disjoint_Included_r. now apply occurs_free_Eprim_Included.
           eapply Union_Disjoint_r. now eauto with Ensembles_DB.
           eapply Disjoint_Singleton_r; eassumption.
-        * eapply binding_not_in_map_antimon; [| eassumption ].
-          normalize_bound_var...
-      + intros x s1. apply return_triple.
-        intros s2 [S' [Hexp Hfr]]. eexists; split; eauto.
+      + intros x s1. apply return_triple. 
+        intros _ [c2 _u] [S' [Hexp Hfr]]. eexists; split; eauto.
         constructor; eauto. rewrite <- rename_not_in_domain_f_eq.
         eassumption.
-        eapply binding_not_in_map_antimon; [| eassumption ].
-        normalize_bound_var...
+        repeat normalize_bound_var_in_ctx. eapply Disjoint_In_l. eassumption. sets.
     - eapply return_triple. intros s1 Hfr. eexists. split; eauto.
       econstructor.
-    - edestruct Hin1 as [[[v' ft'] fvs]  Heq]. now left; eauto.
-      unfold fun_map in Heq. edestruct (M.get v FNmap) eqn:Heq'; try discriminate.
-      destruct f. inv Heq.
-      eapply bind_triple.
-      + eapply add_free_vars_f_eq. eassumption.
-      + intros [ys map'] _. apply pre_curry_l. intros Heq1.
-        apply pre_curry_l. intros Hnin'. apply pre_curry_l. intros Hnd.
-        apply pre_curry_l. intros Hall. apply pre_curry_l. intros Hlen.
-        eapply bind_triple. now eapply get_names_fresh.
-        intros xs' s1. apply pre_curry_l. intros Hall'. apply pre_curry_l. intros Hlen'.
-        apply pre_curry_l. intros Hnd'. eapply bind_triple.
-        * { inv Hun. eapply IHe; eauto.
-            - eapply Disjoint_Included_r; [| eassumption ].
-              normalize_bound_var...
-            - eapply Disjoint_Included_r; [| eassumption ].
-              normalize_bound_var...
-            - eapply Disjoint_Included; [| | eapply Hf ].
-              eapply Union_Included. normalize_bound_var...
-              eapply Included_trans. eapply (occurs_free_in_fun v t l e (Fcons v t l e f5)).
-              now left; eauto.
-              eapply Union_Included. normalize_bound_var...
-              eapply Union_Included. eapply Included_Union_preserv_l.
-              now apply name_in_fundefs_bound_var_fundefs.
-              now eauto with Ensembles_DB. now eauto with Ensembles_DB.
-            - eapply Disjoint_Included_r. eapply (occurs_free_in_fun v t l e (Fcons v t l e f5)).
-              now constructor. eapply Union_Disjoint_r.
-              eassumption. simpl. eapply Union_Disjoint_r. eapply Union_Disjoint_r.
-              eapply Disjoint_Singleton_r. eassumption.
-              eapply Disjoint_Included_r. now apply name_in_fundefs_bound_var_fundefs.
-              eassumption. rewrite bound_var_fundefs_Fcons in HD...
-            - eapply binding_not_in_map_antimon; [| eassumption ].
-              rewrite (Setminus_Disjoint _ (FromList fvs)). normalize_bound_var...
-              eapply Disjoint_Included_r_sym with (s3 := FunsFVs (fun_map FNmap)).
-              intros x H. repeat eexists; eauto. unfold fun_map. rewrite Heq'. reflexivity.
-              eassumption. }
-        * { intros e' s2. eapply pre_existential. intros S1.
-            eapply pre_curry_l. intros Hll.
+    - inv Hun. 
+      repeat normalize_bound_var_in_ctx. repeat normalize_occurs_free_in_ctx. inv Hor.
+      { (* Case Lifted Funs *)
+        edestruct (M.get v FNmap) eqn:Heq'; try discriminate.
+        destruct f.
+        + eapply bind_triple.
+          * eapply add_free_vars_f_eq. eassumption.
+          * destructAll. intros [ys map'] _. apply pre_curry_l. intros Heq1.
+            apply pre_curry_l. intros Hnin1. apply pre_curry_l. intros Hnd.
+            apply pre_curry_l. intros Hall. apply pre_curry_l. intros Hlen.
             eapply bind_triple.
-            - inv Hun. eapply IHB; eauto.
-              + eapply Disjoint_Included_r; [| eassumption ].
-                normalize_bound_var. eapply Included_Union_compat.
-                eapply Included_trans. now eapply Exp_Lambda_lift_free_set_Included; eauto.
-                now eauto with Ensembles_DB. now eauto with Ensembles_DB.
-              + eapply Disjoint_Included_r; [| eassumption ].
-                normalize_bound_var. eapply Included_Union_compat.
-                eapply Included_trans. now eapply Exp_Lambda_lift_free_set_Included; eauto.
-                now eauto with Ensembles_DB. now eauto with Ensembles_DB.
-              + eapply Disjoint_Included; [| | now apply Hf].
-                eapply Union_Included. normalize_bound_var...
-                eapply Included_trans. now apply occurs_free_fundefs_Fcons_Included.
-                normalize_bound_var...
-                eapply Included_trans. now eapply Exp_Lambda_lift_free_set_Included; eauto.
-                now eauto with Ensembles_DB.
-              + eapply Disjoint_Included_r. now apply occurs_free_fundefs_Fcons_Included.
-                eapply Union_Disjoint_r. rewrite bound_var_fundefs_Fcons in HD...
+            eapply make_wrappers_sound_subset. eassumption.
+            intros xs' s1. simpl. destruct xs'. apply pre_existential. intros B'.
+            apply pre_existential. intros sig. eapply pre_existential. intros S'. 
+            eapply pre_curry_l. intro; subst. eapply pre_curry_l. intros Hwr. apply pre_curry_l. intros Hfew.
+            apply pre_curry_l. intros Hfeq'. eapply bind_triple.
+            { eapply IHe; eauto.
+              - eapply Disjoint_Included_r; [| eassumption ]. eapply Make_wrappers_free_set_Included in Hwr.
+                eapply Union_Included; sets. eapply Included_trans. eassumption. sets.
+              - eapply Disjoint_Included_r; [| eassumption ]. eapply Make_wrappers_free_set_Included in Hwr.
+                eapply Union_Included; sets. eapply Included_trans. eassumption. sets.
+              - eapply Disjoint_Included; [| | eapply Hf ].
+                eapply Union_Included. now sets.
+                eapply Included_trans. eapply (occurs_free_in_fun v t l e (Fcons v t l e f5)).
+                now left; eauto.
+                eapply Union_Included. now sets.
+                eapply Union_Included. eapply Included_Union_preserv_l.
+                eapply Included_trans. apply name_in_fundefs_bound_var_fundefs. normalize_bound_var...
+                normalize_occurs_free... eapply Included_trans.
+                eapply Make_wrappers_free_set_Included in Hwr.
+                eassumption. now eauto with Ensembles_DB.
+              - eapply Disjoint_Included_r. eapply (occurs_free_in_fun v t l e (Fcons v t l e f5)).
+                now constructor. eapply Union_Disjoint_r.
+                eassumption. simpl. eapply Union_Disjoint_r. eapply Union_Disjoint_r.
                 eapply Disjoint_Singleton_r. eassumption.
-              + eapply Included_trans; [| eassumption ]...
-              + eapply binding_not_in_map_antimon; [| eassumption ].
-                eapply Included_Union_compat.
-                eapply Included_trans. now eapply Exp_Lambda_lift_free_set_Included; eauto.
-                now eauto with Ensembles_DB.  normalize_bound_var...
-            - intros B' s3. eapply return_triple.
-              intros s4 [S2 [Hll' Hfr]]. eexists; split; eauto.
-              econstructor; try eassumption.
-              + unfold fun_map. rewrite Heq'. reflexivity.
-              + intros x Hl. eapply Forall_forall; [| eassumption ].
-                eapply Forall_monotonic; [| eassumption ]. intros y Hfy.
-                eapply Hfy. zify; omega.
-              + intros x Hl. eapply Forall_forall; [| eassumption ].
-                eapply Forall_monotonic; [| eassumption ]. intros y Hfy.
-                eapply Hfy. zify; omega.
-              + congruence.
-              + rewrite extend_lst_app; eauto.
-                rewrite Heq1; eauto. rewrite <- rename_not_in_domain_lst_f_eq.
-                eassumption.
-                eapply binding_not_in_map_antimon; [| eassumption ].
-                rewrite (Setminus_Disjoint _ (FromList fvs)). normalize_bound_var...
-                eapply Disjoint_Included_r_sym with (s6 := FunsFVs (fun_map FNmap)).
-                intros x H. repeat eexists; eauto. unfold fun_map. rewrite Heq'. reflexivity.
-                eassumption. }
+                eapply Disjoint_Included_r. now apply name_in_fundefs_bound_var_fundefs.
+                eassumption. normalize_occurs_free. sets.
+              - eapply Union_Disjoint_l. eapply Disjoint_Included_l.
+                eapply Make_wrappers_free_set_Included. eassumption. rewrite Hfeq'.
+                eapply Union_Disjoint_r. eapply Disjoint_Included; [| | eapply Hf ].
+                eapply Included_trans. eapply name_in_fundefs_bound_var_fundefs. now sets.
+                now sets.
+                eapply Disjoint_Included_l; [ | eassumption ].
+                rewrite Setminus_Union_distr. rewrite (Setminus_Disjoint S (FromList l1)). now sets.
+                eapply Disjoint_sym. eapply Disjoint_Included; [ | | eapply Hfvs ]. now sets.
+                intros z Hin. do 4 eexists. split. unfold fun_map. rewrite Heq'. reflexivity. eassumption.
+                rewrite Hfeq'. sets. eapply Union_Disjoint_r; sets.
+                eapply Disjoint_Included_l; [| eapply Hdis ].
+                rewrite !Setminus_Union_distr. do 2 eapply Included_Union_preserv_r. eapply Included_Union_preserv_l.
+                rewrite Setminus_Disjoint. now sets. eapply Union_Disjoint_r; sets.
+                eapply Disjoint_Included_r. eapply name_in_fundefs_bound_var_fundefs. eassumption.
+                eapply Disjoint_Included_l; [| eassumption ].
+                rewrite Setminus_Union_distr. rewrite !Setminus_Union_distr. rewrite Setminus_Disjoint with (s2 := bound_var e).
+                now sets. eapply Disjoint_sym. eapply Disjoint_Included; [| | eapply Hfvs ]. now sets.
+                intros el Hel. do 4 eexists. split. unfold Funs, fun_map. rewrite Heq'. now eauto. eassumption.
+              - eapply Disjoint_Included_l; [| eassumption ].
+                rewrite !Setminus_Union_distr. do 2 eapply Included_Union_preserv_r. eapply Included_Union_preserv_l.
+                rewrite Setminus_Disjoint. now sets. eapply Union_Disjoint_r; sets.
+                eapply Disjoint_Included_r. eapply name_in_fundefs_bound_var_fundefs. eassumption. }
+            { intros e' s2. eapply pre_existential. intros S1.
+              eapply pre_curry_l. intros Hll.
+              assert (Hsub : S1 \subset S). 
+              { eapply Included_trans. eapply Exp_Lambda_lift_free_set_Included. eassumption.
+                eapply Included_trans. eapply Make_wrappers_free_set_Included; eauto. now sets. }  
+              eapply bind_triple.
+              - eapply IHB; eauto.
+                + eapply Disjoint_Included_r; [| eassumption ]. xsets.
+                + eapply Disjoint_Included_r; [| eassumption ]. xsets.
+                + eapply Disjoint_Included; [| | now apply Hf].
+                  eapply Union_Included. eapply Union_Included. now sets.
+                  rewrite !Union_assoc. rewrite Union_Setminus_Included with (s5 := [set v]); tci.
+                  now sets. now sets. now sets. eassumption.
+                + eapply Disjoint_Included_l; [| eassumption ].
+                  rewrite !Setminus_Union_distr. do 3 eapply Included_Union_preserv_r.
+                  rewrite <- Setminus_Union. rewrite Setminus_Disjoint with (s4 := [set v]).
+                  now sets. now sets.
+                + eapply Disjoint_Included_r. now apply occurs_free_fundefs_Fcons_Included.
+                  eapply Union_Disjoint_r. eapply Disjoint_Included; [| | eapply HD ].
+                  normalize_occurs_free. now sets. now sets. now sets.
+                + xsets.
+                + eapply Disjoint_Included_l; [| eapply Hnin' ].
+                  rewrite !Setminus_Union_distr. do 3 eapply Included_Union_preserv_r.
+                  rewrite <- Setminus_Union. rewrite Setminus_Disjoint with (s4 := [set v]).
+                  now sets. now sets.
+                + left. split; eauto. eapply Included_trans; [| eapply H ]...
+                + eapply Included_trans; [| eassumption ]...
+              - intros B'' s3. eapply return_triple.
+                intros _ s4 [S2 [Hll' Hfr]]. eexists; split; eauto. intros Hsub'.
+                assert (Hfeq : f_eq ((rename FVmap) <{ l ++ l1 ~> l ++ ys }>) (rename map')).
+                { rewrite extend_lst_app; eauto. rewrite Heq1.
+                  rewrite <- rename_not_in_domain_lst_f_eq. reflexivity.
+                  eapply Disjoint_Included_l; [| eassumption ].
+                  rewrite !Setminus_Union_distr.
+                  rewrite Setminus_Disjoint with (s5 := FromList l). now sets.
+                  eapply Disjoint_sym. eapply Disjoint_Included; [| | eapply Hfvs ]. now sets.
+                  intros el Hel. do 4 eexists. split. unfold Funs, fun_map. rewrite Heq'. now eauto. eassumption. }
+                edestruct Make_wrappers_f_eq. eassumption. symmetry. eassumption. reflexivity.
+                inv H1. 
+                econstructor; try eassumption.
+                + unfold fun_map. rewrite Heq'. reflexivity.
+                + now eauto.
+                + rewrite <- H3, <- Hfew. eassumption.
+                + eapply Hll'. eapply Included_trans; [| eassumption ]...
+                + split. intros Hdis1. exfalso. eapply Hdis1. constructor. now left.
+                  eapply H. now left. eapply Hfr. }
+        + exfalso. destructAll.
+          assert (Hind:  domain (fun_map FNmap) v).
+          { eapply H. now left. }
+          destruct Hind. unfold fun_map in *. rewrite Heq' in *. congruence.
+        + exfalso. destructAll.
+          assert (Hind:  domain (fun_map FNmap) v).
+          { eapply H. now left. }
+          destruct Hind. unfold fun_map in *. rewrite Heq' in *. congruence. }
+      { (* Case No Lifted Funs *)
+        edestruct (M.get v FNmap) eqn:Heq'; try discriminate.
+        destruct f.
+        + exfalso. destructAll. eapply H. constructor; eauto. unfold In, domain.
+          eexists. unfold fun_map. rewrite Heq'. reflexivity.
+        + eapply bind_triple.
+          { eapply IHe; eauto.
+            - sets.
+            - sets.
+            - sets. eapply Disjoint_Included_r; [| eassumption ].
+              eapply Included_trans. eapply bound_var_occurs_free_Fcons_Included.
+              normalize_bound_var. normalize_occurs_free. sets.
+            - eapply fun_in_fundefs_Disjoint_bound_Var_occurs_free with (B := (Fcons v t l e f5)).
+              now left. constructor; eauto.
+              repeat normalize_occurs_free. repeat normalize_bound_var. eassumption.
+            - xsets.
+            - eapply Disjoint_Included_l ; [| eassumption ].
+              rewrite !Setminus_Union_distr. do 2 eapply Included_Union_preserv_r. eapply Included_Union_preserv_l.
+              rewrite Setminus_Disjoint. now sets. eapply Union_Disjoint_r; sets.
+                eapply Disjoint_Included_r. eapply name_in_fundefs_bound_var_fundefs. eassumption. }
+            { intros e' s2. eapply pre_existential. intros S1.
+              eapply pre_curry_l. intros Hll.
+              assert (Hsub : S1 \subset S).
+              { eapply Exp_Lambda_lift_free_set_Included. eassumption. }
+              
+              eapply bind_triple.
+              - eapply IHB; eauto.
+                + sets.
+                + sets.
+                + eapply Disjoint_Included; [| | now apply Hf].
+                  eapply Union_Included. eapply Union_Included. now sets.
+                  rewrite !Union_assoc. rewrite Union_Setminus_Included with (s4 := [set v]); tci.
+                  now sets. now sets. now sets. eassumption.
+                + eapply Disjoint_Included_l; [| eassumption ].
+                  rewrite !Setminus_Union_distr. do 3 eapply Included_Union_preserv_r.
+                  rewrite <- Setminus_Union. rewrite Setminus_Disjoint with (s3 := [set v]).
+                  now sets. now sets.
+                + eapply Disjoint_Included_r. now apply occurs_free_fundefs_Fcons_Included.
+                  eapply Union_Disjoint_r. eapply Disjoint_Included; [| | eapply HD ].
+                  normalize_occurs_free. now sets. now sets. now sets.
+                + now xsets.
+                + eapply Disjoint_Included_l; [| eapply Hnin' ].
+                  rewrite !Setminus_Union_distr. do 3 eapply Included_Union_preserv_r.
+                  rewrite <- Setminus_Union. rewrite Setminus_Disjoint with (s3 := [set v]).
+                  now sets. now sets.
+                + right. inv H. split; eauto. clear H1. now sets.
+                + eapply Included_trans; [| eassumption ]...
+              - intros B'' s3. eapply return_triple.
+                intros _ s4 [S2 [Hll' Hfr]]. eexists; split; eauto.
+                + intros Hsub'. exfalso. inv H. eapply H0. constructor; eauto.
+                + inv Hfr. split; eauto. intros Hdis2. econstructor.
+                  rewrite <- rename_not_in_domain_add_extend_fundefs_f_eq.
+                  2:{ eapply Disjoint_Included_l. eapply name_in_fundefs_bound_var_fundefs. sets. }
+                  rewrite <- rename_not_in_domain_lst_f_eq. eassumption.
+                  now sets. eapply H0. sets. }
+        + exfalso. destructAll.
+          assert (Hind: Dom_map FNmap v).
+          { eapply Hdom. now left. }
+          destruct Hind. congruence. }
     - apply return_triple. intros s1 Hfr. eexists; split; eauto.
-      constructor.
+      intros. constructor.
+      split; intros. constructor. eassumption.
+
+      Grab Existential Variables.
+      eassumption. eassumption. eassumption. 
   Qed.
   
 End Lambda_lifting_corresp.
